Updated version of the confidential and authenticated send and receive functions that reuse existing functions

src/lib/communication/DY.Lib.Communication.API.Lemmas.fst
@@ -8,7 +8,7 @@ open DY.Lib.State.PKI
 open DY.Lib.State.PrivateKeys
 open DY.Lib.Event.Typed
 
-open DY.Lib.Communication.API.Predicates
+open DY.Lib.Communication.API.Invariants
 open DY.Lib.Communication.API
 
 #set-options "--fuel 0 --ifuel 0 --z3cliopt 'smt.qi.eager_threshold=100'"
@@ -18,8 +18,8 @@ open DY.Lib.Communication.API
 val encrypt_message_proof:
   {|cinvs:crypto_invariants|} ->
   tr:trace ->
-  sender:principal -> receiver:principal -> payload:bytes ->
-  pk:bytes -> nonce:bytes ->
+  sender:principal -> receiver:principal -> 
+  pk:bytes -> nonce:bytes -> payload:bytes ->
   Lemma
   (requires
     has_communication_layer_invariants cinvs /\
@@ -30,12 +30,9 @@ val encrypt_message_proof:
     event_triggered tr sender (CommConfSendMsg sender receiver payload)
   )
   (ensures
-    is_publishable tr (encrypt_message sender receiver payload pk nonce)
+    is_publishable tr (encrypt_message pk nonce payload)
   )
-let encrypt_message_proof #cinvs tr sender receiver payload pk nonce =
-  let msg = CM {sender; receiver; payload} in  
-  serialize_wf_lemma communication_message (is_knowable_by (join (principal_label sender) (principal_label receiver)) tr) msg;
-  ()
+let encrypt_message_proof #cinvs tr sender receiver pk nonce payload = ()
 
 val send_confidential_proof:
   {|invs:protocol_invariants|} ->
@@ -48,7 +45,7 @@ val send_confidential_proof:
     trace_invariant tr /\
     has_pki_invariant invs /\
     has_communication_layer_invariants invs.crypto_invs /\
-    comm_higher_layer_event_preds_later tr (higher_layer_preds.send_conf sender receiver payload) /\
+    comm_layer_preds_later tr (higher_layer_preds.send_conf sender receiver payload) /\
     has_communication_layer_event_predicates invs higher_layer_preds /\    
     is_knowable_by (join (principal_label sender) (principal_label receiver)) tr payload
   )
@@ -63,10 +60,10 @@ let send_confidential_proof #invs tr higher_layer_preds keys_sess_ids sender rec
     let (Some pk_receiver, tr) = get_public_key sender keys_sess_ids.pki (PkEnc comm_layer_pkenc_tag) receiver tr in
     let (nonce, tr) = mk_rand PkNonce (principal_label sender) 32 tr in
     let ((), tr) = trigger_event sender (CommConfSendMsg sender receiver payload) tr in
-    let msg_encrypted = encrypt_message sender receiver payload pk_receiver nonce in
+    let msg_encrypted = encrypt_message pk_receiver nonce payload in
     assert(higher_layer_preds.send_conf sender receiver payload tr);
     assert(event_triggered tr sender (CommConfSendMsg sender receiver payload));
-    encrypt_message_proof tr sender receiver payload pk_receiver nonce;
+    encrypt_message_proof tr sender receiver pk_receiver nonce payload;
     let (msg_id, tr) = send_msg msg_encrypted tr in
     assert(tr_out == tr);
     ()
@@ -84,22 +81,20 @@ val decrypt_message_proof:
   )
   (ensures (
     match decrypt_message sk_receiver msg_encrypted with
-    | Some {sender; receiver=receiver'; payload} -> (
-      let Some msg_plain = pk_dec sk_receiver msg_encrypted in
-      (is_knowable_by (join (principal_label sender) (principal_label receiver)) tr payload /\
-        event_triggered tr sender (CommConfSendMsg sender receiver payload)) \/
+    | Some payload -> (
+      (exists sender.
+        get_label sk_receiver == principal_label receiver /\
+        is_knowable_by (join (principal_label sender) (principal_label receiver)) tr payload /\
+        event_triggered tr sender (CommConfSendMsg sender receiver payload)
+      ) \/ (
         is_publishable tr payload
+      )
     )
     | _ -> True
   ))
 let decrypt_message_proof #cinvs tr receiver sk_receiver msg_encrypted =
   match decrypt_message sk_receiver msg_encrypted with
-  | Some {sender; receiver=receiver'; payload} -> ( 
-    let Some msg_plain = pk_dec sk_receiver msg_encrypted in
-    FStar.Classical.move_requires (parse_wf_lemma communication_message (is_publishable tr)) msg_plain;
-    FStar.Classical.move_requires (parse_wf_lemma communication_message (bytes_invariant tr)) msg_plain;
-    ()
-  )
+  | Some payload -> ()
   | _ -> ()
 
 
@@ -114,31 +109,25 @@ val receive_confidential_proof:
     trace_invariant tr /\ 
     has_private_keys_invariant invs /\
     has_communication_layer_invariants invs.crypto_invs /\
-    (
-      match receive_confidential comm_keys_ids receiver msg_id tr with
-      | (None, tr_out) -> True
-      | (Some {sender; receiver=receiver'; payload}, tr_out) ->
-        comm_higher_layer_event_preds_later tr (higher_layer_preds.receive_conf sender receiver payload)
-    ) /\
     has_communication_layer_event_predicates invs higher_layer_preds
   )
   (ensures (
     match receive_confidential comm_keys_ids receiver msg_id tr with
     | (None, tr_out) -> trace_invariant tr_out
-    | (Some {sender; receiver=receiver'; payload}, tr_out) -> ( 
+    | (Some payload, tr_out) -> ( 
       trace_invariant tr_out /\
-      event_triggered tr_out receiver (CommConfReceiveMsg sender receiver payload)
+      event_triggered tr_out receiver (CommConfReceiveMsg receiver payload)
     )
   ))
 let receive_confidential_proof #invs tr higher_layer_preds comm_keys_ids receiver msg_id =
   match receive_confidential comm_keys_ids receiver msg_id tr with
   | (None, tr_out) -> ()
-  | (Some {sender; receiver=receiver'; payload}, tr_out) -> (
+  | (Some payload, tr_out) -> (
     let (Some sk_receiver, tr) = get_private_key receiver comm_keys_ids.private_keys (PkDec comm_layer_pkenc_tag) tr in
     let (Some msg_encrypted, tr) = recv_msg msg_id tr in
     let Some msg_plain = decrypt_message sk_receiver msg_encrypted in
     decrypt_message_proof tr receiver sk_receiver msg_encrypted;
-    let ((), tr) = trigger_event receiver (CommConfReceiveMsg msg_plain.sender receiver msg_plain.payload) tr in
+    let ((), tr) = trigger_event receiver (CommConfReceiveMsg receiver payload) tr in
     assert(tr_out == tr);
     ()
   )
@@ -149,8 +138,8 @@ let receive_confidential_proof #invs tr higher_layer_preds comm_keys_ids receive
 val sign_message_proof:
   {|cinvs:crypto_invariants|} ->
   tr:trace ->
-  sender:principal -> receiver:principal -> payload:bytes ->
-  sk:bytes -> nonce:bytes ->
+  sender:principal -> receiver:principal -> payload:bytes -> is_encrypted:bool ->
+  sk:bytes -> nonce:bytes -> 
   Lemma
   (requires
     has_communication_layer_invariants cinvs /\
@@ -158,19 +147,45 @@ val sign_message_proof:
     is_secret (principal_label sender) tr nonce /\
     SigNonce? (get_usage nonce) /\
     is_signature_key (SigKey comm_layer_sign_tag empty) (principal_label sender) tr sk /\
-    event_triggered tr sender (CommAuthSendMsg sender payload)
+    (
+      if is_encrypted then (
+        (exists plain_msg nonce pk_receiver.
+          //pk_enc_extract_pk payload == Some (DY.Core.Bytes.Type.Pk sk_receiver) /\
+          //Some plain_msg == pk_dec sk_receiver payload /\
+          payload == encrypt_message pk_receiver nonce plain_msg /\
+          //get_label sk_receiver == principal_label receiver /\
+          event_triggered tr sender (CommConfSendMsg sender receiver plain_msg) /\
+          event_triggered tr sender (CommAuthSendMsg sender plain_msg) /\ 
+          event_triggered tr sender (CommConfAuthSendMsg sender receiver plain_msg) /\   
+          get_label plain_msg `can_flow tr` (join (principal_label sender) (principal_label receiver))
+        )
+      ) else (
+        event_triggered tr sender (CommAuthSendMsg sender payload)
+      )
+    )
   )
   (ensures
-    is_publishable tr (sign_message sender receiver payload sk nonce)
+    is_publishable tr (sign_message sender receiver payload is_encrypted sk nonce)
   )
-let sign_message_proof #cinvs tr sender receiver payload sk nonce =
-  let msg = CM {sender; receiver; payload} in
-  serialize_wf_lemma communication_message (is_publishable tr) msg;
-  let msg_bytes = serialize communication_message #parseable_serializeable_bytes_communication_message msg in
-  let signature = sign sk nonce msg_bytes in
-  let msg_signed = CMSign {sender; receiver; payload; signature} in  
-  serialize_wf_lemma communication_message #parseable_serializeable_bytes_communication_message (is_publishable tr) msg_signed;
-  ()
+let sign_message_proof #cinvs tr sender receiver payload is_encrypted sk nonce =
+  if is_encrypted then (
+    let sig_input = Encrypted {sender; receiver; payload} in
+    let sig_input_bytes = serialize signature_input sig_input in
+    serialize_wf_lemma signature_input (is_publishable tr) sig_input;
+    let signature = sign sk nonce sig_input_bytes in
+    let msg_signed = {sender; receiver; payload; signature} in
+    assert(bytes_invariant tr signature);
+    serialize_wf_lemma communication_message_sign (is_publishable tr) msg_signed;
+    ()
+  ) else (
+    let sig_input = Plain {sender; receiver; payload} in
+    let sig_input_bytes = serialize signature_input sig_input in
+    serialize_wf_lemma signature_input (is_publishable tr) sig_input;
+    let signature = sign sk nonce sig_input_bytes in
+    let msg_signed = {sender; receiver; payload; signature} in
+    serialize_wf_lemma communication_message_sign (is_publishable tr) msg_signed;
+    ()
+  )
 
 val send_authenticated_proof:
   {|invs:protocol_invariants|} ->
@@ -182,7 +197,9 @@ val send_authenticated_proof:
   (requires
     trace_invariant tr /\ has_private_keys_invariant invs /\
     has_communication_layer_invariants invs.crypto_invs /\
-    comm_higher_layer_event_preds_later tr (higher_layer_preds.send_auth sender payload) /\
+    //if_comm_conf_payload sender receiver payload tr /\
+    //comm_layer_preds_later tr (if_comm_conf_payload sender receiver payload) /\
+    comm_layer_preds_later tr (higher_layer_preds.send_auth sender payload) /\
     has_communication_layer_event_predicates invs higher_layer_preds /\
     is_publishable tr payload
   )
@@ -198,50 +215,113 @@ let send_authenticated_proof #invs tr higher_layer_preds comm_keys_ids sender re
       let (nonce,  tr) = mk_rand SigNonce (principal_label sender) 32 tr in      
       let ((), tr) = trigger_event sender (CommAuthSendMsg sender payload) tr in
       assert(event_triggered tr sender (CommAuthSendMsg sender payload)); 
-      let msg_signed = sign_message sender receiver payload sk_sender nonce in
-      sign_message_proof tr sender receiver payload sk_sender nonce;
+      let msg_signed = sign_message sender receiver payload false sk_sender nonce in
+      sign_message_proof tr sender receiver payload false sk_sender nonce;
       let (msg_id, tr) = send_msg msg_signed tr in
       assert(tr_out == tr);
       ()
     )
-  
 
-#push-options "--ifuel 1 --fuel 0"
+
 val verify_message_proof:
   {|cinvs:crypto_invariants|} ->
   tr:trace ->
   sender:principal -> receiver:principal ->
-  msg_bytes:bytes -> vk_sender:bytes ->
+  msg_bytes:bytes -> is_encrypted:bool ->
+  vk_sender:bytes ->
   Lemma
   (requires
     has_communication_layer_invariants cinvs /\
     is_publishable tr msg_bytes /\
-    is_verification_key (SigKey comm_layer_sign_tag empty) (principal_label sender) tr vk_sender
+    is_verification_key (SigKey comm_layer_sign_tag empty) (principal_label sender) tr vk_sender    
   )
   (ensures (
-    match verify_message receiver msg_bytes vk_sender with
+    match verify_message receiver msg_bytes is_encrypted vk_sender with
     | Some {sender=sender'; receiver=receiver'; payload} -> (
       is_publishable tr payload /\
-      ((get_signkey_label vk_sender == principal_label sender' /\
-        sender' == sender /\
-        event_triggered tr sender' (CommAuthSendMsg sender' payload)) \/
-        get_signkey_label vk_sender `can_flow tr` public)      
+      (
+        (
+          get_signkey_label vk_sender == principal_label sender /\
+          sender' == sender /\
+          (
+            if is_encrypted then (
+              exists plain_msg nonce pk_receiver.
+                //pk_enc_extract_pk payload == Some (DY.Core.Bytes.Type.Pk sk_receiver) /\
+                //Some plain_msg == decrypt_message sk_receiver payload /\
+                //get_label sk_receiver == principal_label receiver /\
+                payload == encrypt_message pk_receiver nonce plain_msg /\
+                event_triggered tr sender (CommConfSendMsg sender receiver plain_msg) /\
+                event_triggered tr sender (CommAuthSendMsg sender plain_msg) /\
+                event_triggered tr sender (CommConfAuthSendMsg sender receiver plain_msg) /\
+                get_label plain_msg `can_flow tr` (join (principal_label sender) (principal_label receiver))
+            ) else (
+              event_triggered tr sender (CommAuthSendMsg sender payload)
+            )
+          )
+        ) \/ (
+          is_corrupt tr (principal_label sender)
+        )
+      )
     )
     | _ -> True
   ))
-let verify_message_proof #cinvs tr sender receiver msg_bytes vk_sender =
+let verify_message_proof #cinvs tr sender receiver msg_bytes is_encrypted vk_sender =
   assert(get_signkey_label vk_sender == principal_label sender);
-  match verify_message receiver msg_bytes vk_sender with
+  match verify_message receiver msg_bytes is_encrypted vk_sender with
   | Some {sender=sender'; receiver=receiver'; payload} -> (
-    parse_wf_lemma communication_message (is_publishable tr) msg_bytes;
-    let msg = CM {sender=sender'; receiver=receiver'; payload} in
-    serialize_wf_lemma communication_message #parseable_serializeable_bytes_communication_message (is_publishable tr) msg;
-    ()
+    parse_wf_lemma communication_message_sign (is_publishable tr) msg_bytes;
+    //assert(is_publishable tr payload);
+    let Some msg_signed = parse communication_message_sign msg_bytes in
+    
+    //assert(bytes_invariant tr vk_sender);
+    //assert(bytes_invariant tr msg_bytes);
+    //assert(bytes_invariant tr msg_signed.signature);
+    //normalize_term_spec bytes_invariant;
+    //reveal_opaque (`%verify) (verify);
+    
+
+    (*assert(event_triggered tr sender (CommAuthSendMsg sender payload) \/
+      get_signkey_label vk_sender `can_flow tr` public);
+    
+    let DY.Core.Bytes.Type.Sign sk nonce sig_input_bytes = msg_signed.signature in
+    assert(sign_pred.pred tr (Vk sk) sig_input_bytes \/
+      get_signkey_label vk_sender `can_flow tr` public);
+
+    assert(receiver == receiver');
+    assert(sender == sender' \/
+      get_signkey_label vk_sender `can_flow tr` public);*)
+    
+    if is_encrypted then (
+      let sig_input_e = Encrypted {sender=sender'; receiver=msg_signed.receiver; payload=msg_signed.payload} in
+      //let sig_input_bytes_e = serialize signature_input #parseable_serializeable_bytes_signature_input sig_input_e in
+      serialize_wf_lemma signature_input (is_publishable tr) sig_input_e;
+      //assert(verify vk_sender sig_input_bytes_e msg_signed.signature);      
+      //assert(bytes_invariant tr sig_input_bytes_e);      
+      //bytes_invariant_verify tr vk_sender sig_input_bytes_e msg_signed.signature;
+
+      (*let Some sig_input = parse signature_input sig_input_bytes in
+      assert(Encrypted? sig_input);
+      let sig_input_record = Encrypted?.msg sig_input in
+      assert(sign_pred.pred tr (Vk sk) sig_input_bytes \/
+        get_signkey_label vk_sender `can_flow tr` public);
+      assert(msg_signed.receiver == receiver);
+      let sig_input' = Encrypted {sender=sender'; receiver=msg_signed.receiver; payload=msg_signed.payload} in
+      let sig_input_bytes' = serialize signature_input sig_input' in
+      assert(verify vk_sender sig_input_bytes' msg_signed.signature);
+      assert(sig_input_record.sender == sender \/
+        get_signkey_label vk_sender `can_flow tr` public);
+      assert(event_triggered tr sender (CommConfSendMsg sender receiver msg) \/
+        get_signkey_label (Vk sk) `can_flow tr` public);*)
+      ()
+    ) else (
+      let sig_input_p = Plain {sender=sender'; receiver=msg_signed.receiver; payload=msg_signed.payload} in
+      serialize_wf_lemma signature_input (is_publishable tr) sig_input_p;
+      ()
+    )
   )
   | _ -> ()
-#pop-options
 
-val extract_data_from_msg_id:
+(*val extract_data_from_msg_id:
   tr:trace ->
   comm_keys_ids:communication_keys_sess_ids ->
   receiver:principal -> msg_id:timestamp ->
@@ -257,14 +337,14 @@ let extract_data_from_msg_id tr comm_keys_ids receiver msg_id fn =
       match get_public_key receiver comm_keys_ids.pki (Verify comm_layer_sign_tag) sender tr with
       | (None, tr) -> True
       | (Some vk_sender, tr) -> (
-        match verify_message receiver msg_signed vk_sender with
+        match verify_message receiver msg_signed false vk_sender with
         | None -> True
         | Some {sender=sender'; receiver=receiver'; payload} -> (
           fn sender receiver payload
         )
       )
     )
-  )
+  )*)
 
 val receive_authenticated_proof:
   {|invs:protocol_invariants|} ->
@@ -276,37 +356,314 @@ val receive_authenticated_proof:
   (requires
     trace_invariant tr /\ has_pki_invariant invs /\
     has_communication_layer_invariants invs.crypto_invs /\
-    (
-      extract_data_from_msg_id tr comm_keys_ids receiver msg_id (
-        fun sender receiver payload -> (
-          comm_higher_layer_event_preds_later tr (
-            higher_layer_preds.receive_auth sender receiver payload
-          )
-        )
-      )
-    ) /\
     has_communication_layer_event_predicates invs higher_layer_preds
   )
   (ensures (
-    let (_, tr_out) = receive_authenticated comm_keys_ids receiver msg_id tr in
-    trace_invariant tr_out /\
-    (
-      extract_data_from_msg_id tr comm_keys_ids receiver msg_id (
-        fun sender receiver payload ->
-          event_triggered tr_out receiver (CommAuthReceiveMsg sender receiver payload)
-      )
+    match receive_authenticated comm_keys_ids receiver msg_id tr with
+    | (Some {sender; receiver; payload}, tr_out) -> (
+      trace_invariant tr_out /\
+      event_triggered tr_out receiver (CommAuthReceiveMsg sender receiver payload)
     )
+    | (None, tr_out) -> trace_invariant tr_out
   ))
 let receive_authenticated_proof #invs tr higher_layer_preds comm_keys_ids receiver msg_id =
   match receive_authenticated comm_keys_ids receiver msg_id tr with
   | (None, tr_out) -> ()
   | (Some {sender=sender'; receiver=receiver'; payload}, tr_out) -> (
     let (Some msg_signed, tr) = recv_msg msg_id tr in
-    let Some sender = get_sender msg_signed in
-    let (Some vk_sender, tr) = get_public_key receiver comm_keys_ids.pki (Verify comm_layer_sign_tag) sender tr in
-    let (Some msg_bytes, tr) = recv_msg msg_id tr in
-    verify_message_proof tr sender receiver msg_bytes vk_sender;
-    let ((), tr) = trigger_event receiver (CommAuthReceiveMsg sender receiver payload) tr in
+    let Some msg = parse_sig_message msg_signed in
+    let (Some vk_sender, tr) = get_public_key receiver comm_keys_ids.pki (Verify comm_layer_sign_tag) msg.sender tr in
+    verify_message_proof tr msg.sender receiver msg_signed false vk_sender;
+    let ((), tr) = trigger_event receiver (CommAuthReceiveMsg msg.sender receiver payload) tr in
     assert(tr_out == tr);
+    ()
+  )
+
+
+(**** Confidential and Authenticates Send and Receive Lemmas ****)
+
+//#push-options "--ifuel 4 --fuel 4 --z3rlimit 50"
+val encrypt_and_sign_message_proof:
+  {|cinvs:crypto_invariants|} ->
+  tr:trace ->
+  sender:principal -> receiver:principal -> payload:bytes ->
+  pk_receiver:bytes -> sk_sender:bytes -> enc_nonce:bytes -> sign_nonce:bytes ->
+  Lemma
+  (requires
+    has_communication_layer_invariants cinvs /\
+    is_knowable_by (join (principal_label sender) (principal_label receiver)) tr payload /\
+    is_secret (principal_label sender) tr enc_nonce /\
+    is_secret (principal_label sender) tr sign_nonce /\
+    PkNonce? (get_usage enc_nonce) /\
+    SigNonce? (get_usage sign_nonce) /\
+    is_encryption_key (PkKey comm_layer_pkenc_tag empty) (principal_label receiver) tr pk_receiver /\
+    is_signature_key (SigKey comm_layer_sign_tag empty) (principal_label sender) tr sk_sender /\
+    event_triggered tr sender (CommConfSendMsg sender receiver payload) /\
+    event_triggered tr sender (CommAuthSendMsg sender payload) /\
+    event_triggered tr sender (CommConfAuthSendMsg sender receiver payload)
+  )
+  (ensures
+    is_publishable tr (encrypt_and_sign_message sender receiver payload pk_receiver sk_sender enc_nonce sign_nonce)
+  )
+let encrypt_and_sign_message_proof #cinvs tr sender receiver payload pk_receiver sk_sender enc_nonce sign_nonce =
+  encrypt_message_proof #cinvs tr sender receiver pk_receiver enc_nonce payload;
+  let enc_payload = encrypt_message pk_receiver enc_nonce payload in
+  assert(get_label sk_sender == principal_label sender);
+  assert(is_publishable tr enc_payload);
+  assert(enc_payload == encrypt_message pk_receiver enc_nonce payload);
+  assert(event_triggered tr sender (CommConfSendMsg sender receiver payload));
+  assert(event_triggered tr sender (CommAuthSendMsg sender payload));
+  assert(get_label payload `can_flow tr` (join (principal_label sender) (principal_label receiver)));
+  //normalize_term_spec pk_dec;
+  //normalize_term_spec pk_enc;
+  //normalize_term_spec get_sk_label;
+  //normalize_term_spec get_sk_usage;
+  //normalize_term_spec pk;
+
+  (*assert(match pk_receiver with
+  | DY.Core.Bytes.Type.Pk sk -> get_usage sk == PkKey comm_layer_pkenc_tag empty
+  | _ -> False);
+  assert(match pk_receiver with
+  | DY.Core.Bytes.Type.Pk sk -> get_label sk == principal_label receiver
+  | _ -> False);
+
+  assert(is_publishable tr enc_payload);
+
+  assert(enc_payload == pk_enc pk_receiver enc_nonce payload);
+
+  
+    
+  eliminate exists sk_receiver. get_label sk_receiver == principal_label receiver
+  returns exists sk_receiver. pk_dec sk_receiver (pk_enc pk_receiver enc_nonce payload) == Some payload
+  with _. (
+    pk_dec_enc sk_receiver enc_nonce payload;
+    assert(
+        pk_dec sk_receiver (pk_enc (pk sk_receiver) enc_nonce payload) == Some payload
+    );
+    assert(Some payload == decrypt_message sk_receiver enc_payload);
+    assert(exists plain_msg.
+      Some plain_msg == decrypt_message sk_receiver enc_payload
+    );
+    assert(exists plain_msg.
+      get_label plain_msg `can_flow tr` (join (principal_label sender) (principal_label receiver)));
+
+    
+
+    assert(has_communication_layer_invariants cinvs /\
+      is_publishable tr enc_payload /\
+      is_secret (principal_label sender) tr sign_nonce /\
+      SigNonce? (get_usage sign_nonce) /\
+      is_signature_key (SigKey comm_layer_sign_tag empty) (principal_label sender) tr sk_sender /\
+      (
+        if true then (
+          (exists sk_receiver plain_msg.
+            Some plain_msg == pk_dec sk_receiver enc_payload /\
+            get_label sk_receiver == principal_label receiver /\
+            event_triggered tr sender (CommConfSendMsg sender receiver plain_msg) /\
+            event_triggered tr sender (CommAuthSendMsg sender plain_msg) /\      
+            get_label plain_msg `can_flow tr` (join (principal_label sender) (principal_label receiver))
+          )
+        ) else (
+          event_triggered tr sender (CommAuthSendMsg sender payload)
+        )
+      ));
+    sign_message_proof tr sender receiver enc_payload true sk_sender sign_nonce;
+    ()
+  );*)
+  
+  sign_message_proof tr sender receiver enc_payload true sk_sender sign_nonce;
+  ()
+
+
+val send_confidential_authenticated_proof:
+  {|invs:protocol_invariants|} ->
+  tr:trace ->
+  higher_layer_preds:comm_higher_layer_event_preds ->
+  comm_keys_ids:communication_keys_sess_ids ->
+  sender:principal -> receiver:principal -> payload:bytes ->
+  Lemma
+  (requires
+    trace_invariant tr /\
+    has_private_keys_invariant invs /\
+    has_pki_invariant invs /\
+    has_communication_layer_invariants invs.crypto_invs /\
+    comm_layer_preds_later tr (higher_layer_preds.send_conf sender receiver payload) /\
+    comm_layer_preds_later tr (higher_layer_preds.send_auth sender payload) /\
+    comm_layer_preds_later tr (higher_layer_preds.send_conf_auth sender receiver payload) /\
+    has_communication_layer_event_predicates invs higher_layer_preds /\
+    is_knowable_by (join (principal_label sender) (principal_label receiver)) tr payload
+  )
+  (ensures (
+    let (_, tr_out) = send_confidential_authenticated comm_keys_ids sender receiver payload tr in
+    trace_invariant tr_out
+  ))
+let send_confidential_authenticated_proof #invs tr higher_layer_preds comm_keys_ids sender receiver payload =
+  match send_confidential_authenticated comm_keys_ids sender receiver payload tr with
+  | (None, tr_out) -> ()
+  | (Some _, tr_out) -> (
+    let (Some pk_receiver, tr) = get_public_key sender comm_keys_ids.pki (PkEnc comm_layer_pkenc_tag) receiver tr in
+    let (Some sk_sender, tr) = get_private_key  sender comm_keys_ids.private_keys (Sign comm_layer_sign_tag) tr in
+    let (enc_nonce, tr) = mk_rand PkNonce (principal_label sender) 32 tr in
+    let (sign_nonce, tr) = mk_rand SigNonce (principal_label sender) 32 tr in
+    let ((), tr) = trigger_event sender (CommConfSendMsg sender receiver payload) tr in
+    let ((), tr) = trigger_event sender (CommAuthSendMsg sender payload) tr in
+    assert(event_triggered tr sender (CommConfSendMsg sender receiver payload));
+    assert(event_triggered tr sender (CommAuthSendMsg sender payload));
+    let ((), tr) = trigger_event sender (CommConfAuthSendMsg sender receiver payload) tr in
+    assert(event_triggered tr sender (CommConfAuthSendMsg sender receiver payload));
+    encrypt_and_sign_message_proof tr sender receiver payload pk_receiver sk_sender enc_nonce sign_nonce;
+    let msg = encrypt_and_sign_message sender receiver payload pk_receiver sk_sender enc_nonce sign_nonce in
+    let (msg_id, tr) = send_msg msg tr in
+    assert(tr_out == tr);
+    ()
+  )
+
+
+val verify_and_decrypt_message_proof:
+  {|cinvs:crypto_invariants|} ->
+  tr:trace ->
+  sender:principal -> receiver:principal -> msg_encrypted_signed:bytes ->
+  sk_receiver:bytes -> vk_sender:bytes ->
+  Lemma
+  (requires
+    has_communication_layer_invariants cinvs /\
+    is_publishable tr msg_encrypted_signed /\
+    is_verification_key (SigKey comm_layer_sign_tag empty) (principal_label sender) tr vk_sender /\
+    is_decryption_key (PkKey comm_layer_pkenc_tag empty) (principal_label receiver) tr sk_receiver
+  )
+  (ensures (
+    match verify_and_decrypt_message receiver msg_encrypted_signed sk_receiver vk_sender with
+    | None -> True
+    | Some {sender=sender'; receiver=receiver'; payload} -> (
+    (
+      let Some sig_msg = parse_sig_message msg_encrypted_signed in 
+      get_signkey_label vk_sender == principal_label sender /\
+      sender' == sender /\
+      event_triggered tr sender (CommAuthSendMsg sender payload) /\
+      is_knowable_by (join (principal_label sender) (principal_label receiver)) tr payload /\
+      event_triggered tr sender (CommConfSendMsg sender receiver payload) /\
+      event_triggered tr sender (CommConfAuthSendMsg sender receiver payload)
+    ) \/
+      is_corrupt tr (principal_label sender)
+    )
+  ))
+let verify_and_decrypt_message_proof #cinvs tr sender receiver msg_encrypted_signed sk_receiver vk_sender =
+  match verify_and_decrypt_message receiver msg_encrypted_signed sk_receiver vk_sender with
+  | None -> ()
+  | Some {sender=sender'; receiver=receiver'; payload} -> (
+    verify_message_proof tr sender receiver msg_encrypted_signed true vk_sender;
+    let Some {sender=sender''; receiver=receiver''; payload=enc_payload} = verify_message receiver msg_encrypted_signed true vk_sender in    
+    assert(is_publishable tr enc_payload /\
+      (
+        (
+          get_signkey_label vk_sender == principal_label sender /\
+          sender' == sender /\
+          (exists plain_msg nonce pk_receiver.
+            //pk_enc_extract_pk enc_payload == Some (DY.Core.Bytes.Type.Pk sk_receiver) /\
+            //Some plain_msg == decrypt_message sk_receiver enc_payload /\
+            //get_label sk_receiver == principal_label receiver /\
+            enc_payload == encrypt_message pk_receiver nonce plain_msg /\
+            event_triggered tr sender (CommConfSendMsg sender receiver plain_msg) /\
+            event_triggered tr sender (CommAuthSendMsg sender plain_msg) /\
+            get_label plain_msg `can_flow tr` (join (principal_label sender) (principal_label receiver))
+          )
+        ) \/ (
+          is_corrupt tr (principal_label sender)
+        )
+      )
+    );
+
+    decrypt_message_proof tr receiver sk_receiver enc_payload;
+    let Some payload' = decrypt_message sk_receiver enc_payload in
+    normalize_term_spec pk_dec;
+    normalize_term_spec pk_enc;
+    //assert(pk_enc_extract_pk enc_payload == Some (DY.Core.Bytes.Type.Pk sk_receiver));
+    assert(payload == payload');
+    assert((exists sender. 
+        get_label sk_receiver == principal_label receiver /\
+        is_knowable_by (join (principal_label sender) (principal_label receiver)) tr payload /\
+        event_triggered tr sender (CommConfSendMsg sender receiver payload)
+      ) \/ (
+        is_publishable tr payload
+      )
+    );
+
+    ()
+    (*introduce ~(is_corrupt tr (principal_label sender)) /\ ~(is_publishable tr payload) ==> event_triggered tr sender (CommConfSendMsg sender receiver payload)
+    with _. (
+      assert(exists payload. event_triggered tr sender (CommConfSendMsg sender receiver payload));
+      eliminate exists plain_msg. event_triggered tr sender (CommConfSendMsg sender receiver plain_msg)
+      returns event_triggered tr sender (CommConfSendMsg sender receiver payload)
+      with _. (
+        assert(
+          event_triggered tr sender (CommAuthSendMsg sender payload) /\
+          is_knowable_by (join (principal_label sender) (principal_label receiver)) tr payload /\
+          event_triggered tr sender (CommConfSendMsg sender receiver payload)
+        );
+        ()
+      )
+    )*)
+    (*reveal_opaque (`%pk_enc) (pk_enc);
+    reveal_opaque (`%pk_dec) (pk_dec);
+    let DY.Core.Bytes.Type.PkEnc pk nonce msg = enc_payload in
+    assert(if_comm_conf_payload sender receiver'' enc_payload tr \/
+      is_corrupt tr (principal_label sender));
+    assert(get_usage sk_receiver == PkKey comm_layer_pkenc_tag empty);
+    assert(Pk sk_receiver == pk);
+    reveal_opaque (`%get_sk_usage) (get_sk_usage);
+    assert(get_sk_usage pk == PkKey comm_layer_pkenc_tag empty);
+    assert(
+      (
+        get_sk_label pk == principal_label receiver'' /\
+        event_triggered tr sender (CommConfSendMsg sender receiver'' msg)
+      ) \/
+        is_corrupt tr (principal_label sender)                                                        
+    );
+    assert(get_label sk_receiver == principal_label receiver);
+    assert(get_sk_label pk == principal_label receiver'' \/
+      is_corrupt tr (principal_label sender));
+    reveal_opaque (`%get_sk_label) (get_sk_label);
+    assert(receiver == receiver'' \/
+      is_corrupt tr (principal_label sender));
+    decrypt_message_proof tr receiver sk_receiver enc_payload;*)
+  )
+
+val receive_confidential_authenticated_proof:
+  {|invs:protocol_invariants|} ->
+  tr:trace ->
+  higher_layer_preds:comm_higher_layer_event_preds ->
+  comm_keys_ids:communication_keys_sess_ids ->
+  receiver:principal -> msg_id:timestamp ->
+  Lemma
+  (requires
+    trace_invariant tr /\
+    has_private_keys_invariant invs /\
+    has_pki_invariant invs /\
+    has_communication_layer_invariants invs.crypto_invs /\
+    has_communication_layer_event_predicates invs higher_layer_preds
+  )
+  (ensures
+    (
+      match receive_confidential_authenticated comm_keys_ids receiver msg_id tr with
+      | (None, tr_out) -> trace_invariant tr_out
+      | (Some {sender; receiver=receiver'; payload}, tr_out) -> (
+        trace_invariant tr_out /\
+        event_triggered tr_out receiver (CommConfAuthReceiveMsg sender receiver payload)
+      )
+    )
+  )
+let receive_confidential_authenticated_proof #invs tr higher_layer_preds comm_keys_ids receiver msg_id =
+  match receive_confidential_authenticated comm_keys_ids receiver msg_id tr with
+  | (None, tr_out) -> ()
+  | (Some {sender; receiver=receiver'; payload}, tr_out) -> (
+    let (Some msg_encrypted_signed, tr) = recv_msg msg_id tr in
+    let Some msg_sig = parse_sig_message msg_encrypted_signed in
+    let (Some sk_receiver, tr) = get_private_key receiver comm_keys_ids.private_keys (PkDec comm_layer_pkenc_tag) tr in
+    let (Some vk_sender, tr) = get_public_key receiver comm_keys_ids.pki (Verify comm_layer_sign_tag) msg_sig.sender tr in
+    let Some msg = verify_and_decrypt_message receiver msg_encrypted_signed sk_receiver vk_sender in
+    verify_and_decrypt_message_proof tr sender receiver msg_encrypted_signed sk_receiver vk_sender;
+    let ((), tr) = trigger_event receiver (CommConfAuthReceiveMsg msg.sender receiver msg.payload) tr in
+    assert(event_triggered tr receiver (CommConfAuthReceiveMsg msg.sender receiver msg.payload));
+    assert(tr == tr_out);
     ()
   )
